Common/Values.v
@@ -10,76 +10,92 @@ Module Block.
   Definition local : id := 0.
 End Block.
 
-Module Pointer.
-  Definition t : Type := Component.id * Block.id * Block.offset.
+Module Permission.
+  Definition id := nat.
+  Definition code : id := 0.
+  Definition data : id := 1.
+End Permission.
 
+Module Pointer.
+  Definition t : Type := Permission.id * Component.id * Block.id * Block.offset.
+
+  Definition permission (p : t) : Permission.id :=
+    let '(P, _, _, _) := p in P.
+  
   Definition component (p : t) : Component.id :=
-    let '(C, _, _) := p in C.
+    let '(_, C, _, _) := p in C.
 
   Definition block (p : t) : Block.id :=
-    let '(_, b, _) := p in b.
+    let '(_, _, b, _) := p in b.
 
   Definition offset (p : t) : Block.offset :=
-    let '(_, _, o) := p in o.
+    let '(_, _, _, o) := p in o.
 
   Definition eq (p1 p2 : t) : bool :=
-    let '(C1, b1, o1) := p1 in
-    let '(C2, b2, o2) := p2 in
-    (Nat.eqb C1 C2) && (Nat.eqb b1 b2) && (Z.eqb o1 o2).
+    let '(P1, C1, b1, o1) := p1 in
+    let '(P2, C2, b2, o2) := p2 in
+    (Nat.eqb P1 P2) && (Nat.eqb C1 C2) && (Nat.eqb b1 b2) && (Z.eqb o1 o2).
 
   Definition leq (p1 p2 : t) : option bool :=
-    let '(C1, b1, o1) := p1 in
-    let '(C2, b2, o2) := p2 in
-    if (Nat.eqb C1 C2) && (Nat.eqb b1 b2) then
+    let '(P1, C1, b1, o1) := p1 in
+    let '(P2, C2, b2, o2) := p2 in
+    if (Nat.eqb P1 P2) && (Nat.eqb C1 C2) && (Nat.eqb b1 b2) then
       Some ((o1 <=? o2) % Z)
     else
       None.
 
   Definition add (ptr : t) (offset : Z) : t :=
-    let '(C, b, o) := ptr in (C, b, (o+offset)%Z).
+    let '(P, C, b, o) := ptr in (P, C, b, (o+offset)%Z).
 
   Definition sub (ptr : t) (offset : Z) : t :=
-    let '(C, b, o) := ptr in (C, b, (o-offset)%Z).
+    let '(P, C, b, o) := ptr in (P, C, b, (o-offset)%Z).
 
   Definition inc (ptr : t) : t := add ptr 1.
 
+  Ltac preserves_proof_add := intros ?p ?n; destruct p as [[[P C] b] o]; reflexivity.
+  Ltac preserves_proof_inc := intros ?p; destruct p as [[[P C] b] o]; reflexivity.
+  
+  Lemma add_preserves_permission:
+    forall p n, permission (add p n) = permission p.
+  Proof. preserves_proof_add. Qed.
+
   Lemma add_preserves_component:
     forall p n, component (add p n) = component p.
-  Proof.
-    intros p n.
-    destruct p as [[C b] o].
-    reflexivity.
-  Qed.
-
+  Proof. preserves_proof_add. Qed.
+  
   Lemma add_preserves_block:
     forall p n, block (add p n) = block p.
-  Proof.
-    intros p n.
-    destruct p as [[C b] o].
-    reflexivity.
-  Qed.
+  Proof. preserves_proof_add. Qed.
+
+  Lemma sub_preserves_permission:
+    forall p n, permission (sub p n) = permission p.
+  Proof. preserves_proof_add. Qed.
+
+  Lemma sub_preserves_component:
+    forall p n, component (sub p n) = component p.
+  Proof. preserves_proof_add. Qed.
+  
+  Lemma sub_preserves_block:
+    forall p n, block (sub p n) = block p.
+  Proof. preserves_proof_add. Qed.
+
+  Lemma inc_preserves_permission:
+    forall p, permission (inc p) = permission p.
+  Proof. preserves_proof_inc. Qed.
 
   Lemma inc_preserves_component:
     forall p, component (inc p) = component p.
-  Proof.
-    intros p.
-    destruct p as [[C b] o].
-    reflexivity.
-  Qed.
-
+  Proof. preserves_proof_inc. Qed.
+  
   Lemma inc_preserves_block:
     forall p, block (inc p) = block p.
-  Proof.
-    intros p.
-    destruct p as [[C b] o].
-    reflexivity.
-  Qed.
+  Proof. preserves_proof_inc. Qed.
 
   Lemma compose :
     forall ptr,
-      (component ptr, block ptr, offset ptr) = ptr.
+      (permission ptr, component ptr, block ptr, offset ptr) = ptr.
   Proof.
-    now intros [[C b] o].
+    now intros [[[P C] b] o].
   Qed.
 End Pointer.
 
@@ -100,7 +116,7 @@ Definition eqvalue v1 v2 :=
 
 Lemma eqvalueP : Equality.axiom eqvalue.
 Proof.
-  move; elim => [z1 | p1 |] [z2 | p2|]//= ;
+  move; elim => [z1 | p1 |] [z2 | p2 |]//= ;
                  apply: (iffP idP); move => H; inversion H ; try constructor.
   by move: H => /Z.eqb_spec => H; rewrite H.
   done.
@@ -122,12 +138,12 @@ Definition eval_binop (op : binop) (v1 v2 : value) : value :=
   | Mul,   Int n1, Int n2 => Int (n1 * n2)
   | Eq,    Int n1, Int n2 => Int (Util.Z.of_bool (n1  =? n2)%Z)
   | Leq,   Int n1, Int n2 => Int (Util.Z.of_bool (n1 <=? n2)%Z)
-  (* pointer arithmetic *)
+  (* data-pointer arithmetic *)
   | Add,   Ptr p,  Int n  => Ptr (Pointer.add p n)
   | Add,   Int n,  Ptr p  => Ptr (Pointer.add p n)
-  | Minus, Ptr p1, Ptr p2 => let '(C1, b1, o1) := p1 in
-                             let '(C2, b2, o2) := p2 in
-                             if (Nat.eqb C1 C2) && (Nat.eqb b1 b2) then
+  | Minus, Ptr p1, Ptr p2 => let '(P1, C1, b1, o1) := p1 in
+                             let '(P2, C2, b2, o2) := p2 in
+                             if (Nat.eqb P1 P2) && (Nat.eqb C1 C2) && (Nat.eqb b1 b2) then
                                Int (o1 - o2)
                              else
                                Undef
