S2I/Compiler.v
@@ -279,8 +279,12 @@ Definition compile_components
         do blocks <- lift (local_buffers C);
         do _ <- lift (blocks local_buffer_block_id );
         do P_labels <- lift (procs_labels C);
-        do procs_code <- compile_procedures C (C, local_buffer_block_id, 0%Z) P_labels
-                                            (elementsm procs);
+        do procs_code <- compile_procedures C
+           (Permission.code, C, local_buffer_block_id, 0%Z)
+           (* Used Permission.code here. 
+              Not sure though if it matters here which permission is used. *)
+           P_labels
+           (elementsm procs);
         let acc' := (C, mkfmap procs_code) :: acc in
         compile acc' cs'
       end
